src/QUIC.Spec.Old.fsti
@@ -1,9 +1,10 @@
-module QUIC.Spec
-include QUIC.Parse
+module QUIC.Spec.Old
 
 module S = FStar.Seq
 module HD = Spec.Hash.Definitions
 module AEAD = Spec.Agile.AEAD
+
+type byte = FStar.UInt8.t
 
 // JP: should we allow inversion on either hash algorithm or AEAD algorithm?
 #set-options "--max_fuel 0 --max_ifuel 0"
@@ -18,6 +19,9 @@ let supported_aead = function
 
 type ha = a:HD.hash_alg{supported_hash a}
 type ea = a:AEAD.alg{supported_aead a}
+
+type bytes = s:S.seq byte
+type lbytes (n:nat) = b:bytes{S.length b = n}
 
 // Move from Hashing.Spec to Spec.Hash?
 let keysized (a:ha) (l:nat) =
@@ -40,6 +44,7 @@ let max_cipher_length : n:nat {
 
 type pbytes = b:bytes{let l = S.length b in 3 <= l /\ l < max_plain_length}
 type cbytes = b:bytes{let l = S.length b in 19 <= l /\ l < max_cipher_length}
+type packet = b:bytes{let l = S.length b in 21 <= l /\ l < pow2 32}
 
 // JP: this is Spec.Agile.Cipher.key_length
 let ae_keysize (a:ea) =
@@ -76,41 +81,142 @@ type nat62 = n:nat{n < pow2 62}
 let add3 (n:nat4) : n:nat{n=0 \/ (n >= 4 /\ n <= 18)} = if n = 0 then 0 else 3+n
 let sub3 (n:nat{n = 0 \/ (n >= 4 /\ n <= 18)}) : nat4 = if n = 0 then 0 else n-3
 type qbytes (n:nat4) = lbytes (add3 n)
+type vlsize = n:nat{n == 1 \/ n == 2 \/ n == 4 \/ n == 8}
+type npn = b:bytes{1 <= S.length b /\ S.length b <= 4}
+
+let vlen (n:nat62) : vlsize =
+  if n < pow2 6 then 1
+  else if n < pow2 14 then 2
+  else if n < pow2 30 then 4
+  else 8
+
+val encode_varint: n:nat62 -> lbytes (vlen n)
+val parse_varint: b:bytes -> option (n:nat62 * bytes)
+
+val lemma_varint: (n:nat62) -> (suff:bytes) ->
+  Lemma (parse_varint S.(encode_varint n @| suff) == Some (n,suff))
+
+
+type header =
+  | Short:
+    spin: bool ->
+    phase: bool ->
+    cid:bytes{let l = S.length cid in l == 0 \/ (4 <= l /\ l <= 18)} ->
+    header
+  | Long:
+    typ: nat2 ->
+    version: nat32 ->
+    dcil: nat4 ->
+    scil: nat4 ->
+    dcid: qbytes dcil ->
+    scid: qbytes scil ->
+    len: nat{len < max_cipher_length} ->
+    header
+
+type h_result =
+| H_Success:
+  npn: npn ->
+  h: header ->
+  c: cbytes ->
+  h_result
+| H_Failure
 
 // JP: seems appropriate for this module...?
 let _: squash (inversion header) = allow_inversion header
+
+let header_len (h:header) (pn_len:nat2) : n:nat{2 <= n /\ n <= 54} =
+  match h with
+  | Short spin phase cid ->
+    1 + S.length cid + 1 + pn_len
+  | Long is_hs version dcil scil dcid scid plen ->
+    let _ = assert_norm(max_cipher_length < pow2 62) in
+    6 + add3 dcil + add3 scil + vlen plen + 1 + pn_len
+
+let cid_len : header -> nat4 = function
+  | Short _ _ cid -> sub3 (S.length cid)
+  | Long _ _ dcil _ _ _ _ -> dcil
+
+val format_header: h:header -> npn:npn ->
+  lbytes (header_len h (S.length npn-1))
+
+val parse_header: b:packet -> cid_len: nat4 -> h_result
+
+val lemma_header_parsing_correct:
+  h: header ->
+  npn: npn ->
+  c: cbytes{Long? h ==> S.length c = Long?.len h} ->
+  Lemma (
+    parse_header S.(format_header h npn @| c) (cid_len h)
+    == H_Success npn h c)
+
+// N.B. this is only true for a given DCID len
+val lemma_header_parsing_safe: b1:packet -> b2:packet -> cl:nat4 -> Lemma
+  (requires parse_header b1 cl = parse_header b2 cl)
+  (ensures parse_header b1 cl = H_Failure \/ b1 = b2)
 
 // Header protection only
 val header_encrypt: a:ea ->
   hpk: lbytes (ae_keysize a) ->
   h: header ->
+  npn: npn ->
   c: cbytes ->
-  GTot bytes // packet
+  packet
 
 // Note that cid_len cannot be parsed from short headers
 val header_decrypt: a:ea ->
   hpk: lbytes (ae_keysize a) ->
-  cid_len: nat ->
-  p: bytes -> // packet
-  GTot h_result
-
-module P = QUIC.Parse
+  cid_len: nat4 ->
+  p: packet ->
+  h_result
 
 // This is just functional correctness, but does not guarantee security:
 // decryption can succeed on an input that is not the encryption
-// of the same arguments (see QUIC.Spec.Old.*_malleable)
+// of the same arguments (see next lemma)
 val lemma_header_encryption_correct:
   a:ea ->
   k:lbytes (ae_keysize a) ->
-  h:header { ~ (is_retry h) } ->
-  c: cbytes (* {MLong? h ==> S.length c = MLong?.len h} *) ->
+  h:header ->
+  npn:npn ->
+  c: cbytes{Long? h ==> S.length c = Long?.len h} ->
   Lemma (
-    header_decrypt a k (dcid_len h) (header_encrypt a k h c)
-    == H_Success h c)
+    header_decrypt a k (cid_len h) (header_encrypt a k h npn c)
+    == H_Success npn h c)
 
-noeq
+
+// insert bytes x in b at position i
+val insert : x:bytes -> b:bytes -> i:nat -> Pure bytes
+  (requires i < S.length b)
+  (ensures fun res ->
+    S.length res = S.length b + S.length x /\ (
+    forall j.
+      (j < i ==> S.index res j = S.index b j) /\
+      ((i <= j /\ j < i + S.length x) ==> S.index res j = S.index x (j-i)) /\
+      (i + S.length x <= j ==> S.index res j = S.index b (j-S.length x))))
+
+
+// Even though parse_header is a secure parser, decryption is malleable:
+// it is possible to successfully decrypt while parsing part of the
+// encrypted npn into the cid
+val lemma_header_encryption_malleable:
+  a:ea ->
+  k:lbytes (ae_keysize a) ->
+  c:cbytes ->
+  spin:bool -> phase:bool ->
+  cid:lbytes 4 -> // Arbitrary cid (minimal size to simplify the proof)
+  x: byte -> // Arbitrary part of the npn, transferred to the cid (after xor)
+  npn:byte -> // Rest of the npn
+  y: byte -> // Arbitrary byte, inserted by the adversay in the encrypted header
+  Lemma (
+    let p = header_encrypt a k (Short spin phase cid) S.(create 1 x @| create 1 npn) c in
+    let p' = insert (S.create 1 y) p 7 in
+    S.length p' < pow2 32 /\
+    (exists h' npn'. header_decrypt a k 2 p' = H_Success npn' h' c))
+
+
+
 type result =
-| Success: 
+| Success: pn_len:nat2 ->
+  pn: nat62 ->
   h: header ->
   plain: pbytes ->
   result
@@ -121,8 +227,10 @@ val encrypt:
   k: lbytes (AEAD.key_length a) ->
   static_iv: lbytes 12 ->
   hpk: lbytes (ae_keysize a) ->
+  pn_len: nat2 ->
+  pn: nat62 ->
   h: header ->
-  plain: pbytes (* {Long? h ==> Long?.len h == S.length plain + AEAD.tag_length a} *) ->
+  plain: pbytes{Long? h ==> Long?.len h == S.length plain + AEAD.tag_length a} ->
   packet
 
 
@@ -163,7 +271,7 @@ val decrypt:
   static_iv: lbytes 12 ->
   hpk: lbytes (ae_keysize a) ->
   last: nat{last+1 < pow2 62} ->
-  cid_len: nat ->
+  cid_len: nat4 ->
   packet: packet ->
   result
 
@@ -172,11 +280,13 @@ val lemma_encrypt_correct:
   k: lbytes (AEAD.key_length a) ->
   siv: lbytes 12 ->
   hpk: lbytes (ae_keysize a) ->
+  pn_len: nat2 ->
+  pn: nat62 ->
   last: nat{last+1 < pow2 62} ->
   h: header ->
-  p: pbytes (* {Long? h ==> Long?.len h == S.length p + AEAD.tag_length a} *) -> Lemma
-  (requires True) // in_window pn_len last pn)
+  p: pbytes{Long? h ==> Long?.len h == S.length p + AEAD.tag_length a} -> Lemma
+  (requires in_window pn_len last pn)
   (ensures
-    decrypt a k siv hpk last (dcid_len h)
-      (encrypt a k siv hpk h p)
-    == Success h p)
+    decrypt a k siv hpk last (cid_len h)
+      (encrypt a k siv hpk pn_len pn h p)
+    == Success pn_len pn h p)
