src/QUIC.Parse.VarInt.fsti
@@ -1,17 +1,9 @@
 module QUIC.Parse.VarInt
+include QUIC.Spec.Base
 
 module U64 = FStar.UInt64
 module LP = LowParse.Spec.BoundedInt // for bounded_int32
 module LL = LowParse.Low.Base
-
-inline_for_extraction
-let varint_bound : (varint_bound: U64.t { U64.v varint_bound == pow2 62 }) =
-  [@inline_let] let v = 4611686018427387904uL in
-  [@inline_let] let _ = assert_norm (U64.v v == pow2 62) in
-  v
-
-inline_for_extraction
-let varint_t = (x: U64.t { U64.v x < U64.v varint_bound })
 
 inline_for_extraction
 let parse_varint_kind = {
@@ -70,3 +62,4 @@ val serialize_bounded_varint_impl
   (min: nat)
   (max: nat { min <= max /\ max < 4294967296 })
 : Tot (LL.serializer32 (serialize_bounded_varint min max))
+
