src/QUIC.Spec.Lemmas.fst
@@ -1,0 +1,585 @@
+module QUIC.Spec.Lemmas
+open QUIC.Spec.Base
+
+module S = FStar.Seq
+module U8 = FStar.UInt8
+
+(* library lemmas *)
+
+let suffix (b:bytes) (n:nat{n <= S.length b}) = S.slice b n (S.length b)
+
+let max (a b:int) : Tot (n:int{n >= a /\ n >= b}) =
+  if a > b then a else b // this must exist somewhere...
+
+// Move to FStar.Math.Lemmas?
+let lemma_mod_pow2 (a:nat) (b:nat) : Lemma
+  (requires a >= b) (ensures pow2 a % pow2 b == 0)
+  [SMTPat (pow2 a % pow2 b)]
+  =
+  let open FStar.Math.Lemmas in
+  lemma_div_mod (pow2 a) (pow2 b);
+  pow2_minus a b;
+  pow2_plus b (a-b)
+
+let lemma_divrem2 (k:nat) (a:nat) (n:nat)
+  : Lemma (requires a >= k /\ n < pow2 k)
+  (ensures ((pow2 a + n) % pow2 k == n /\ (pow2 a + n) / pow2 k == pow2 (a - k)))
+  =
+  let open FStar.Math.Lemmas in
+  let open FStar.Mul in
+  modulo_distributivity (pow2 a) n (pow2 k);
+  small_mod n (pow2 k);
+  lemma_div_mod (pow2 a + n) (pow2 k);
+  pow2_minus a k
+
+// We really should have this pattern already...
+let lemma_mod0 (x:pos) : Lemma (0 % x == 0)
+  [SMTPat (0 % x)] = ()
+
+// Move to FStar.Math.Lemmas?
+let lemma_pow2_div (a:nat) (b:nat) (k:nat)
+  : Lemma (requires a >= k /\ b >= k)
+    (ensures (pow2 a + pow2 b) / pow2 k == pow2 (a - k) + pow2 (b - k))
+  =
+  let open FStar.Math.Lemmas in
+  let open FStar.Mul in
+  pow2_plus k (b - k);
+  division_addition_lemma (pow2 a) (pow2 k) (pow2 (b-k));
+  pow2_minus b k;
+  pow2_minus a k
+
+#restart-solver
+
+#push-options "--z3rlimit 128"
+
+// FIXME(adl) this proof is very flacky
+// Will be replaced by varint combinator, using bitfield for first 2 bits
+let lemma_divrem3 (k:nat) (a:nat) (b:nat) (n:nat)
+  : Lemma (requires a >= k /\ b >= k /\ n < pow2 k)
+  (ensures (pow2 a + pow2 b + n) % pow2 k == n /\ (pow2 a + pow2 b + n) / pow2 k == pow2 (a - k) + pow2 (b - k))
+  =
+  let open FStar.Math.Lemmas in
+  let open FStar.Mul in
+  modulo_distributivity (pow2 a + pow2 b) n (pow2 k);
+  modulo_distributivity (pow2 a) (pow2 b) (pow2 k);
+  small_mod n (pow2 k);
+  lemma_div_mod (pow2 a + pow2 b + n) (pow2 k);
+  lemma_pow2_div a b k
+
+#pop-options
+
+let lemma_pow2_div2 (a:nat) (b:nat) (c:nat)
+  : Lemma ((a / pow2 b) / pow2 c == a / (pow2 (c + b)))
+  =
+  let open FStar.Math.Lemmas in
+  pow2_plus b c;
+  division_multiplication_lemma a (pow2 b) (pow2 c)
+
+let lemma_div_sub_small (l:nat) (n:nat) (x:nat)
+  : Lemma (requires l > 1)
+  (ensures (n - n % pow2 8) / pow2 (8 `op_Multiply` (l-1)) == n / pow2 (8 `op_Multiply` (l-1)))
+  =
+  let open FStar.Math.Lemmas in
+  let open FStar.Mul in
+  lemma_mod_spec n (pow2 8);
+  lemma_pow2_div2 n 8 (8*(l-2));
+  lemma_pow2_div2 (n - n % pow2 8) 8 (8*(l-2))
+
+#push-options "--z3rlimit 20"
+let rec lemma_be_index (l:pos) (n:nat{n < pow2 (8 `op_Multiply` l)})
+  : Lemma (ensures U8.v (S.index (FStar.Endianness.n_to_be l n) 0)
+    == n / pow2 (8 `op_Multiply` (l-1)))
+    (decreases %[l])
+  =
+  let open FStar.Endianness in
+  let open FStar.Mul in
+  let b = n_to_be l n in
+  let b0 = S.index b 0 in
+  reveal_be_to_n b;
+  if l = 1 then ()
+  else
+    let b1 = S.last b in
+    let b' = S.slice b 0 (l-1) in
+    let b0' = S.index b' 0 in
+    reveal_be_to_n b';
+    assert(U8.v b1 == n % pow2 8);
+    lemma_be_to_n_is_bounded b';
+    lemma_be_index (l-1) (be_to_n b');
+    lemma_pow2_div2 (n - U8.v b1) 8 (8 * (l-1) - 8);
+    lemma_div_sub_small l n (U8.v b1)
+#pop-options
+
+
+let lemma_be_index_bytes (l:pos) (b:bytes) : Lemma
+  (requires S.length b >= l)
+  (ensures FStar.Endianness.be_to_n (S.slice b 0 l) / pow2 (8 `op_Multiply` (l-1)) = U8.v (S.index b 0)) =
+  let open FStar.Endianness in
+  let n = be_to_n (S.slice b 0 l) in
+  lemma_be_to_n_is_bounded (S.slice b 0 l);
+  lemma_be_index l n;
+  n_to_be_be_to_n l (S.slice b 0 l)
+
+
+/// generic lemmas for sequences
+
+let append_slices1 (#a:eqtype) (s1 s2:S.seq a) : Lemma
+  (S.equal s1 (S.slice (S.append s1 s2) 0 (S.length s1))) =
+  ()
+
+let append_slices2 (#a:eqtype) (s1 s2:S.seq a) : Lemma
+  (Seq.equal s2 (Seq.slice (Seq.append s1 s2) (Seq.length s1) (Seq.length s1 + Seq.length s2))) =
+  ()
+
+let append_slices3 (#a:eqtype) (s1 s2:S.seq a) : Lemma
+  ( (forall (i:nat) (j:nat).
+                i <= j /\ j <= Seq.length s2 ==>
+                Seq.equal (Seq.slice s2 i j)
+                          (Seq.slice (Seq.append s1 s2) (Seq.length s1 + i) (Seq.length s1 + j)))) =
+  ()
+
+let lemma_create_slice b i : Lemma
+  (requires S.length b >= i)
+  (ensures S.(equal (create 1 (index b i)) (slice b i (i+1)))) =
+  ()
+
+let lemma_append_assoc (#a:eqtype) (u v w:S.seq a) : Lemma
+  (S.equal S.(u @| v @| w) S.((u @| v) @| w)) =
+  ()
+
+let compose_split (#a:eqtype) (b:S.seq a) (i j:nat) : Lemma
+  (requires i+j <= S.length b)
+  (ensures snd (S.split (snd (S.split b i)) j) = snd (S.split b (i+j))) =
+  ()
+
+let lemma_compose_slice (#a:eqtype) (b:S.seq a) (i j k l:nat) : Lemma
+  (requires i <= j /\ j <= S.length b /\ k <= l /\ k <= j - i /\ l <= j - i)
+  (ensures S.slice (S.slice b i j) k l = S.slice b (i+k) (i+l)) =
+  ()
+
+let add_offset (#a:eqtype) (b:S.seq a) (i:nat) (p1 p2:S.seq a) : Lemma
+  (requires i <= S.length b /\ S.slice b i (S.length b) = S.(p1@|p2))
+  (ensures (
+    assert (S.length S.(p1@|p2) = S.length p1+S.length p2);
+    S.slice b (i+S.length p1) (S.length b) = p2)) =
+  assert (S.length S.(p1@|p2) = S.length p1+S.length p2);
+  append_slices2 p1 p2;
+  compose_split b i (S.length p1)
+
+let slice_trans (#a:eqtype) (b:S.seq a) (i j k:nat) : Lemma
+  (requires i <= j /\ j <= k /\ k <= S.length b)
+  (ensures S.slice b i k = S.(slice b i j @| slice b j k)) =
+  S.lemma_split (S.slice b i k) (j-i)
+
+let extensionality_slice (#a:eqtype) (b1 b2:S.seq a) (i j:nat) : Lemma
+  (requires
+    S.length b1 = S.length b2 /\
+    i <= j /\ j <= S.length b1 /\
+    (forall (k:nat{i<=k /\ k<j}). S.index b1 k = S.index b2 k))
+  (ensures S.equal (S.slice b1 i j) (S.slice b2 i j)) =
+  let index_slice_aux (b:S.seq a) (i j k:nat) : Lemma
+    (requires i <= j /\ j <= S.length b /\ k < j - i)
+    (ensures S.index (S.slice b i j) k = S.index b (i+k)) =
+    () in
+  let index_slice (b:S.seq a{j <= S.length b}) (k:nat{k < j - i}) : Lemma
+    (S.index (S.slice b i j) k = S.index b (i+k)) =
+    index_slice_aux b i j k in
+
+  FStar.Classical.forall_intro (index_slice b1);
+  FStar.Classical.forall_intro (index_slice b2)
+
+
+// application of a byte operation at a subposition
+let rec pointwise_op (#a:eqtype) (f:a->a->a) (b1 b2:S.seq a) (pos:nat) : Pure (S.seq a)
+  (requires S.length b2 + pos <= S.length b1)
+  (ensures fun b -> S.length b == S.length b1)
+  (decreases (S.length b2)) =
+  if b2 = S.empty then b1
+  else
+    let _ = S.lemma_empty b2 in
+    let x = f (S.index b1 pos) (S.index b2 0) in
+    pointwise_op f (S.upd b1 pos x) (S.slice b2 1 (S.length b2)) (pos + 1)
+
+
+// three lemmas to recover indexes after application of bitwise_op
+let rec pointwise_index1 (#a:eqtype) (f:a->a->a) (b1 b2:S.seq a) (i pos:nat) : Lemma
+  (requires (S.length b2 + pos <= S.length b1 /\ i < pos))
+  (ensures (S.index (pointwise_op f b1 b2 pos) i = S.index b1 i))
+  (decreases (S.length b2)) =
+  if b2 = S.empty then ()
+  else begin
+    S.lemma_empty b2;
+    let x = f (S.index b1 pos) (S.index b2 0) in
+    assert (pointwise_op f b1 b2 pos = pointwise_op f (S.upd b1 pos x) (S.slice b2 1 (S.length b2)) (pos + 1));
+    S.lemma_index_upd2 b1 pos x i;
+    assert (S.index (S.upd b1 pos x) i = S.index b1 i);
+    pointwise_index1 f (S.upd b1 pos x) (S.slice b2 1 (S.length b2)) i (pos + 1)
+  end
+
+
+let rec pointwise_index2 (#a:eqtype) (f:a->a->a) (b1 b2:S.seq a) (i pos:nat) : Lemma
+  (requires (S.length b2 + pos <= S.length b1 /\ pos <= i /\ i < S.length b2 + pos))
+  (ensures (S.index (pointwise_op f b1 b2 pos) i = f (S.index b1 i) (S.index b2 (i-pos))))
+  (decreases (S.length b2)) =
+  if S.empty = b2 then ()
+  else begin
+    let x = f (S.index b1 pos) (S.index b2 0) in
+    assert (pointwise_op f b1 b2 pos = pointwise_op f (S.upd b1 pos x) (S.slice b2 1 (S.length b2)) (pos+1));
+    if i = pos then begin
+      pointwise_index1 f (S.upd b1 pos x) (S.slice b2 1 (S.length b2)) pos (pos+1);
+      S.lemma_index_upd1 b1 pos x
+    end
+    else
+      pointwise_index2 f (S.upd b1 pos x) (S.slice b2 1 (S.length b2)) i (pos+1)
+  end
+
+
+let rec pointwise_index3 (#a:eqtype) (f:a->a->a) (b1 b2:S.seq a) (i pos:nat) : Lemma
+  (requires (S.length b2 + pos <= i /\ i < S.length b1))
+  (ensures (S.index (pointwise_op f b1 b2 pos) i = S.index b1 i))
+  (decreases (S.length b2)) =
+  if S.empty = b2 then ()
+  else begin
+    S.lemma_empty b2;
+    let x = f (S.index b1 pos) (S.index b2 0) in
+    pointwise_index3 f (S.upd b1 pos x) (S.slice b2 1 (S.length b2)) i (pos+1)
+  end
+
+
+
+let pointwise_op_suff (#a:eqtype) (f:a->a->a) (a1 a2 b:S.seq a) (pos:nat) : Lemma
+  (requires pos >= S.length a1 /\ S.length b + pos <= S.length a1 + S.length a2)
+  (ensures
+    S.equal
+      (pointwise_op f S.(a1 @| a2) b pos)
+      S.(a1 @| pointwise_op f a2 b (pos - S.length a1))) =
+  let b1 = pointwise_op f S.(a1 @| a2) b pos in
+  let b2 = S.(a1 @| pointwise_op f a2 b (pos - S.length a1)) in
+  let step i : Lemma (S.index b1 i = S.index b2 i) =
+    if i < S.length a1 then pointwise_index1 f S.(a1 @| a2) b i pos
+    else begin
+      if i < pos then begin
+        pointwise_index1 f S.(a1 @| a2) b i pos;
+        pointwise_index1 f a2 b (i-S.length a1) (pos-S.length a1)
+      end else if i < S.length b + pos then begin
+        pointwise_index2 f S.(a1 @| a2) b i pos;
+        pointwise_index2 f a2 b (i-S.length a1) (pos-S.length a1)
+      end else begin
+        pointwise_index3 f S.(a1 @| a2) b i pos;
+        pointwise_index3 f a2 b (i-S.length a1) (pos-S.length a1)
+      end
+    end in
+
+  FStar.Classical.forall_intro step
+
+
+let pointwise_op_pref (#a:eqtype) (f:a->a->a) (a1 a2 b:S.seq a) (pos:nat) : Lemma
+  (requires S.length b + pos <= S.length a1)
+  (ensures
+    S.equal
+      (pointwise_op f S.(a1 @| a2) b pos)
+      S.(pointwise_op f a1 b pos @| a2)) =
+  let b1 = pointwise_op f S.(a1 @| a2) b pos in
+  let b2 = S.(pointwise_op f a1 b pos @| a2) in
+  let step i : Lemma (S.index b1 i = S.index b2 i) =
+    if i < pos then begin
+      pointwise_index1 f S.(a1 @| a2) b i pos;
+      pointwise_index1 f a1 b i pos
+    end else if i < S.length b + pos then begin
+      pointwise_index2 f S.(a1 @| a2) b i pos;
+      pointwise_index2 f a1 b i pos
+    end else begin
+      pointwise_index3 f S.(a1 @| a2) b i pos;
+      if i < S.length a1 then pointwise_index3 f a1 b i pos
+      else ()
+    end in
+
+  FStar.Classical.forall_intro step
+
+
+let pointwise_op_dec (#a:eqtype) (f:a->a->a) (a1 a2 b:S.seq a) (pos:nat) : Lemma
+  (requires
+    pos < S.length a1 /\
+    S.length a1 <= S.length b + pos /\
+    S.length b + pos <= S.length a1 + S.length a2)
+  (ensures (
+    let open S in
+    let (b1,b2) = S.split b (length a1 - pos) in
+    equal
+      (pointwise_op f (a1 @| a2) b pos)
+      (pointwise_op f a1 b1 pos @| pointwise_op f a2 b2 0))) =
+  let open S in
+  let (b1,b2) = S.split b (length a1 - pos) in
+  let p = pointwise_op f (a1 @| a2) b pos in
+  let q = pointwise_op f a1 b1 pos @| pointwise_op f a2 b2 0 in
+  let step i : Lemma (S.index p i = S.index q i) =
+    if i < pos then begin
+      pointwise_index1 f (a1 @| a2) b i pos;
+      pointwise_index1 f a1 b1 i pos
+    end else if i < length a1 then begin
+      pointwise_index2 f (a1 @| a2) b i pos;
+      pointwise_index2 f a1 b1 i pos
+    end else if i < length b + pos then begin
+      pointwise_index2 f (a1 @| a2) b i pos;
+      pointwise_index2 f a2 b2 (i-length a1) 0
+    end else begin
+      pointwise_index3 f (a1 @| a2) b i pos;
+      pointwise_index3 f a2 b2 (i-length a1) 0
+    end in
+
+  FStar.Classical.forall_intro step
+
+
+
+// application: byte-wise xor
+let xor_inplace (b1 b2:bytes) (pos:nat)
+  : Pure bytes
+  (requires S.length b2 + pos <= S.length b1)
+  (ensures fun b -> S.length b == S.length b1)
+  (decreases (S.length b2)) =
+  pointwise_op U8.logxor b1 b2 pos
+
+
+// proof of involution of the operator (uses extensionality for the
+// byte-wise variant)
+let xor_involutive (b1 b2:byte) : Lemma
+  (requires True)
+  (ensures (b1 `U8.logxor` b2) `U8.logxor` b2 = b1) =
+  FStar.UInt.logxor_associative (U8.v b1) (U8.v b2) (U8.v b2);
+  FStar.UInt.logxor_self (U8.v b2);
+  FStar.UInt.logxor_commutative (FStar.UInt.zero 8) (U8.v b1);
+  FStar.UInt.logxor_lemma_1 (U8.v b1)
+
+
+let rec xor_inplace_involutive (b1 b2:bytes) (pos:nat) : Lemma
+  (requires S.length b2 + pos <= S.length b1)
+  (ensures S.equal (xor_inplace (xor_inplace b1 b2 pos) b2 pos) b1)
+  (decreases (S.length b2)) =
+  let xor = xor_inplace (xor_inplace b1 b2 pos) b2 pos in
+  let step (i:nat{i < S.length b1}) : Lemma (S.index xor i = S.index b1 i) =
+    if i < pos then begin
+      pointwise_index1 U8.logxor b1 b2 i pos;
+      pointwise_index1 U8.logxor (xor_inplace b1 b2 pos) b2 i pos
+    end else if i >= pos+S.length b2 then begin
+      pointwise_index3 U8.logxor b1 b2 i pos;
+      pointwise_index3 U8.logxor (xor_inplace b1 b2 pos) b2 i pos
+    end else begin
+      pointwise_index2 U8.logxor b1 b2 i pos;
+      pointwise_index2 U8.logxor (xor_inplace b1 b2 pos) b2 i pos;
+      xor_involutive  (S.index b1 i) (S.index b2 (i-pos))
+    end in
+
+  FStar.Classical.forall_intro step
+
+
+let rec xor_inplace_commutative (b b1 b2:bytes) (pos1 pos2:nat) : Lemma
+  (requires
+    S.length b1 + pos1 <= S.length b /\
+    S.length b2 + pos2 <= S.length b)
+  (ensures S.equal
+    (xor_inplace (xor_inplace b b1 pos1) b2 pos2)
+    (xor_inplace (xor_inplace b b2 pos2) b1 pos1)) =
+  let xor1 = xor_inplace (xor_inplace b b1 pos1) b2 pos2 in
+  let xor2 = xor_inplace (xor_inplace b b2 pos2) b1 pos1 in
+  let step (i:nat{i < S.length b}) : Lemma (S.index xor1 i = S.index xor2 i) =
+    if i < pos1 then begin
+      pointwise_index1 U8.logxor b b1 i pos1;
+      pointwise_index1 U8.logxor (xor_inplace b b2 pos2) b1 i pos1;
+      if i < pos2 then begin
+        pointwise_index1 U8.logxor b b2 i pos2;
+        pointwise_index1 U8.logxor (xor_inplace b b1 pos1) b2 i pos2
+      end else if i >= pos2 + S.length b2 then begin
+        pointwise_index3 U8.logxor b b2 i pos2;
+        pointwise_index3 U8.logxor (xor_inplace b b1 pos1) b2 i pos2
+      end else begin
+        pointwise_index2 U8.logxor b b2 i pos2;
+        pointwise_index2 U8.logxor (xor_inplace b b1 pos1) b2 i pos2
+      end
+    end else if i >= pos1 + S.length b1 then begin
+      pointwise_index3 U8.logxor b b1 i pos1;
+      pointwise_index3 U8.logxor (xor_inplace b b2 pos2) b1 i pos1;
+      if i < pos2 then begin
+        pointwise_index1 U8.logxor b b2 i pos2;
+        pointwise_index1 U8.logxor (xor_inplace b b1 pos1) b2 i pos2
+      end else if i >= pos2 + S.length b2 then begin
+        pointwise_index3 U8.logxor b b2 i pos2;
+        pointwise_index3 U8.logxor (xor_inplace b b1 pos1) b2 i pos2
+      end else begin
+        pointwise_index2 U8.logxor b b2 i pos2;
+        pointwise_index2 U8.logxor (xor_inplace b b1 pos1) b2 i pos2
+      end
+    end else begin
+      pointwise_index2 U8.logxor b b1 i pos1;
+      pointwise_index2 U8.logxor (xor_inplace b b2 pos2) b1 i pos1;
+      if i < pos2 then begin
+        pointwise_index1 U8.logxor b b2 i pos2;
+        pointwise_index1 U8.logxor (xor_inplace b b1 pos1) b2 i pos2
+      end else if i >= pos2 + S.length b2 then begin
+        pointwise_index3 U8.logxor b b2 i pos2;
+        pointwise_index3 U8.logxor (xor_inplace b b1 pos1) b2 i pos2
+      end else begin
+        let ind = U8.v (S.index b i) in
+        let ind1 = U8.v (S.index b1 (i-pos1)) in
+        let ind2 = U8.v (S.index b2 (i-pos2)) in
+        FStar.UInt.logxor_associative #8 ind ind1 ind2;
+        FStar.UInt.logxor_associative #8 ind ind2 ind1;
+        FStar.UInt.logxor_commutative #8 ind1 ind2;
+        pointwise_index2 U8.logxor b b2 i pos2;
+        pointwise_index2 U8.logxor (xor_inplace b b1 pos1) b2 i pos2
+      end
+    end in
+
+  FStar.Classical.forall_intro step
+
+
+let and_inplace (b1 b2:bytes) (pos:nat)
+  : Pure bytes
+  (requires S.length b2 + pos <= S.length b1)
+  (ensures fun b -> S.length b == S.length b1)
+  (decreases (S.length b2)) =
+  pointwise_op U8.logand b1 b2 pos
+
+let rec bitwise_op (f:bool->bool->bool) (l1 l2:list bool) : Pure (list bool)
+  (requires List.Tot.length l1 = List.Tot.length l2)
+  (ensures fun l -> List.Tot.length l = List.Tot.length l1) =
+  match l1,l2 with
+  | [],[] -> []
+  | x1::t1,x2::t2 -> f x1 x2 :: bitwise_op f t1 t2
+
+
+let rec lemma_bitwise_op_index (f:bool->bool->bool) (l1 l2:list bool) (n:nat) : Lemma
+  (requires List.Tot.length l1 = List.Tot.length l2 /\ n < List.Tot.length l1)
+  (ensures List.Tot.index (bitwise_op f l1 l2) n = f (List.Tot.index l1 n) (List.Tot.index l2 n)) =
+  match l1,l2 with
+  | [],[] -> ()
+  | x1::t1,x2::t2 ->
+    if n = 0 then ()
+    else lemma_bitwise_op_index f t1 t2 (n-1)
+
+let rec list_to_seq (#a:eqtype) (l:list a) : (s:(S.seq a){S.length s = List.Tot.length l /\ (forall i. S.index s i = List.Tot.index l i)}) =
+  match l with
+  | [] -> S.empty
+  | h :: t -> S.(create 1 h @| list_to_seq t)
+
+let rec rev_seq (#a:eqtype) (s:S.seq a) : Pure (S.seq a)
+  (requires True)
+  (ensures fun s' -> S.length s = S.length s')
+  (decreases (S.length s)) =
+  if s = S.empty then S.empty
+  else
+    let _ = S.lemma_empty s in
+    S.(rev_seq S.(slice s 1 (length s)) @| create 1 (index s 0))
+
+
+let rec lemma_rev_seq (#a:eqtype) (s:S.seq a) (i:nat) : Lemma
+  (requires i < S.length s)
+  (ensures
+    S.length (rev_seq s) = S.length s /\
+    S.index s i = S.index (rev_seq s) (S.length s-1-i))
+  (decreases (i))=
+  if s = S.empty then ()
+  else if i = 0 then ()
+  else lemma_rev_seq (S.slice s 1 (S.length s)) (i-1)
+
+#restart-solver
+
+let lemma_arithmetic1 (a b c d e:int) : Lemma
+  ((a+b+c+d)+(e-d) = (a+c+e)+b) =
+  ()
+
+let lemma_arithmetic2 (a b c d:int) : Lemma
+  (a+(b-c)+d = a + ((b+d)-c)) =
+  ()
+
+let lemma_arithmetic3 (a b c:int) : Lemma
+  ((a+b)-c = (a-c)+b) =
+  ()
+
+
+let lemma_propagate_mul_mod (a b:nat) : Lemma
+  (requires b > 0)
+  (ensures (
+    let open FStar.Mul in
+    (2*a) % (2*b) = 2 * (a % b))) =
+  let open FStar.Math.Lemmas in
+  let open FStar.Mul in
+  lemma_div_mod a b;
+  lemma_div_mod (2*a) b;
+  let (p,r) = ((a/b)*(2*b), 2*(a%b)) in
+  assert (2*a = p + r);
+  modulo_distributivity p r (2*b);
+  multiple_modulo_lemma (a/b) (2*b);
+  modulo_range_lemma a b;
+  small_mod r (2*b)
+
+#push-options "--max_fuel 2 --initial_fuel 2 --max_ifuel 1 --initial_ifuel 1 --z3rlimit 128" // strange that F* has so much trouble completing this induction
+let recompose_pow2_assoc (n:pos) (a:nat) : Lemma
+  (let open FStar.Mul in 2 * (pow2 (n-1) * a) = pow2 n * a) =
+  ()
+
+
+let rec lemma_propagate_pow_mod (a b n:nat) : Lemma
+  (requires b > 0)
+  (ensures (
+    let open FStar.Mul in
+    (pow2 n * a) % (pow2 n * b) = pow2 n * (a % b))) =
+  let open FStar.Mul in
+  let open FStar.Math.Lemmas in
+  if n = 0 then ()
+  else begin
+    let res = (pow2 n * a) % (pow2 n * b) in
+    lemma_propagate_mul_mod (pow2 (n-1) * a) (pow2 (n-1) * b);
+    assert (res = 2 * ((pow2 (n-1) * a) % (pow2 (n-1) * b)));
+    lemma_propagate_pow_mod a b (n-1);
+    assert (res = 2 * (pow2 (n-1) * (a%b)));
+    recompose_pow2_assoc n (a%b)
+  end
+#pop-options
+
+
+#restart-solver
+let lemma_modulo_shift_byte (a:nat) (i:pos) : Lemma
+  (let open FStar.Mul in
+  (pow2 8 * a) % (pow2 (8*i)) = pow2 8 * (a % pow2 (8*(i-1)))) =
+  let sub = 8 `op_Multiply` (i-1) in
+  FStar.Math.Lemmas.pow2_plus 8 sub;
+  lemma_propagate_pow_mod a (pow2 sub) 8
+
+let rec reveal_be_to_n_slice (b:bytes) (i j:nat) : Lemma
+  (requires i < j /\ j <= S.length b)
+  (ensures (
+    let open FStar.Mul in
+    let open FStar.Endianness in
+    let h = U8.v (S.index b (j-1)) in
+    be_to_n (S.slice b i j) = h + pow2 8 * be_to_n (S.slice b i (j - 1)))) =
+  FStar.Endianness.reveal_be_to_n (S.slice b i j)
+
+let rec lemma_correctness_slice_be_to_n (b:bytes) (i:nat) : Lemma
+  (requires i <= S.length b)
+  (ensures (
+    let open FStar.Endianness in
+    let open FStar.Mul in
+    be_to_n b % pow2 (8 * i) =
+    be_to_n (S.slice b (S.length b - i) (S.length b))))
+  (decreases i) =
+  let open FStar.Endianness in
+  let open FStar.Math.Lemmas in
+  let open FStar.Mul in
+  if i = 0 then reveal_be_to_n S.empty
+  else begin
+    reveal_be_to_n b;
+    let h = U8.v (S.index b (S.length b - 1)) in
+    let l = S.slice b 0 (S.length b - 1) in
+    let pow = pow2 (8*i) in
+    //assert (be_to_n b = h + pow2 8 * be_to_n l);
+    modulo_distributivity h (pow2 8 * be_to_n l) pow;
+    pow2_le_compat (8*i) 8;
+    small_mod h pow;
+    //assert (be_to_n b % pow = (h + (pow2 8 * be_to_n l)%pow) % pow);
+    lemma_modulo_shift_byte (be_to_n l) i;
+    lemma_correctness_slice_be_to_n l (i-1);
+    //assert (be_to_n b % pow = (h + pow2 8 * be_to_n (S.slice b (S.length b - i) (S.length b - 1))) % pow);
+    reveal_be_to_n_slice b (S.length b - i) (S.length b);
+    //assert (be_to_n b % pow = be_to_n (S.slice b (S.length b - i) (S.length b)) % pow);
+    lemma_be_to_n_is_bounded (S.slice b (S.length b - i) (S.length b));
+    FStar.Math.Lemmas.small_mod (be_to_n (S.slice b (S.length b - i) (S.length b))) pow
+  end
